{
 "cells": [
  {
   "cell_type": "markdown",
   "metadata": {},
   "source": [
    "# Simple random walk"
   ]
  },
  {
   "cell_type": "markdown",
   "metadata": {},
   "source": [
    "## One dimensional"
   ]
  },
  {
   "cell_type": "markdown",
   "metadata": {},
   "source": [
    "**Video lecture: https://youtu.be/ere9BtMLoTc**"
   ]
  },
  {
   "cell_type": "markdown",
   "metadata": {},
   "source": [
    "Think of a drunk man, standing out side a bar, walk one step at a time, either left or right, with certain probability. Will he eventually return to the origin state 0? Or thereâ€™s a chance that he will never returns? \n",
    "\n",
    "What's the average time he returns back to the bar? On average, will be be back in 10 steps, 100 steps? 1000 steps?\n",
    "\n",
    "\n",
    "### Time Homogeneity Property\n",
    "\n",
    "Give any $i, j \\in S$, $P(X_{n+1}=j | X_n=i) = P(X_1=j | X_0=i)$ for any $n$. That is no matter how much time parsed, the probability of moving from state $i$ to $j$ never changed.\n",
    "\n",
    "### Spatial Homogeneity Property\n",
    "\n",
    "It's not only time homogeneous but also state homogeneous. i.e. $P(X_{n+1}=j+k | X_n=i+k) = P(X_1=j | X_0=i)$\n",
    "\n",
    "### Theorem: Average moving speed\n",
    "\n",
    "$\\{ X_n, X_n \\in \t\\mathbb{Z}, n \\in \\mathbb{Z^+} \\}$, Let $Z_i$ be iid bernoulli taking value $1$ with probability $p$ and $-1$ with $1-p$, therefore, $\\displaystyle{X_n = \\sum_{i=0}^n{Z_i}}$, by strong law of large numbers, \n",
    "\n",
    "$$\n",
    "\\frac{X_n}{n} \\rightarrow E[Z_0] \\qquad \\text{a.s}\n",
    "$$\n",
    "\n",
    "Where $E[Z_0] = (1)p+(-1)(1-p) = 2p-1$. $E[Z_0]$ defines the average speed it moves. If $E[Z_0] = 0$, it doesn't move away from 0 on average, otherwise, it moves away from 0 in average speed $E[Z_0]$.\n",
    "\n",
    "### Irreducible\n",
    "\n",
    "Since all states are communicate, it's a irreducible markov chain. It can be proved that if state $0$ is recurrent, then all states are recurrent. If $0$ is transient then all states are transient.\n",
    "\n",
    "\n",
    "Our goal is to determine whether state $0$ is transient or recurrent. We are also interested to if expected time of first return is finite or infinite.\n",
    "\n",
    "#### Method 1: Binomial\n",
    "\n",
    "Since it needs even number of steps to return back to zero, therefore:\n",
    "\n",
    "$$\n",
    "\\boldsymbol{P}_{00}^{2n-1} = 0\n",
    "$$\n",
    "\n",
    "$\\boldsymbol{P}_{00}^{2n} = \\binom{2n}{n}p^n(1-p)^n$, using stirling formula $n! \\sim n^{n+1/2}e^{-n}\\sqrt{2\\pi}$:\n",
    "\n",
    "$$\n",
    "\\boldsymbol{P}_{00}^{2n} \\sim \\frac{(4p(1-p))^n}{\\sqrt{\\pi{n}}}\n",
    "$$\n",
    "\n",
    "$$\n",
    "\\displaystyle \\sum_{n=1}{\\boldsymbol{P}_{00}^{2n}} \\sim \\sum_{n=1}{\\frac{(4p(1-p))^n}{\\sqrt{\\pi{n}}}}\n",
    "$$\n",
    "\n",
    "if $p=\\frac{1}{2}$, since $\\sum{\\frac{1}{\\sqrt{n}}}$ is divergent, $\\displaystyle \\sum_{n=1}{\\boldsymbol{P}_{00}^{2n}}=\\infty$, therefore $\\rho_{00} = P_0(T_0 \\lt \\infty) = 1$. \n",
    "Otherwise, $(4p(1-p))^n \\lt 1$, therefore $\\displaystyle \\sum_{n=1}{\\boldsymbol{P}_{00}^{2n}} \\lt \\infty$, therefore $\\rho_{00} = P_0(T_0 \\lt \\infty) \\lt 1$ \n",
    "\n",
    "\n",
    "#### Method 2: Generating function\n",
    "\n",
    "Let $\\rho_{0r}(n) = P(T_r = n| X_0 = 0)$.\n",
    "\n",
    "$$\n",
    "\\begin{aligned}\n",
    "  P_0(T_0 \\lt \\infty) &= \\sum_{n = 0}^{\\infty}{P_0(T_0 = n)} = \\sum_{n = 0}^{\\infty}{\\rho_{00}(n)} \\\\\n",
    "  E_0[T_0] &= \\sum_{n=0}^{\\infty}{nP_0(T_0 = n)} = \\sum_{n=0}^{\\infty}{n\\rho_{00}(n)}\n",
    "\\end{aligned}\n",
    "$$\n",
    "\n",
    "**Definition:** Probability generating function of discrete random variable $X$: $G_{X}(s) = E[s^X] = \\sum_{n=0}^{\\infty}{s^nP(X=n)}$.\n",
    "\n",
    "$$\n",
    "\\begin{aligned}\n",
    "  G_{T_0}(1) &= P_0(T_0 \\lt \\infty)\\\\\n",
    "  G_{T_0}'(1) &= E_0[T_0] \\\\\n",
    "  P(T_0 = n) &= \\frac{1}{n!} G_{T_0}^{(n)}(0)\n",
    "\\end{aligned}\n",
    "$$\n",
    "\n",
    "Therefore, the generating function determines the probability distribution.\n",
    "\n",
    "We want to know $G_{T_0}(1)=\\sum_{n=0}^{\\infty}\\rho_{00}(n) = \\rho_{00}$ is equal to $1$ or $\\lt 1$. We'll find in three steps:\n",
    "\n",
    "- First find $G_{T_r}(s)$ for $r \\gt 1$.\n",
    "- Then use $G_{T_r}(s)$ to find $G_{T_1}(s)$.\n",
    "- Last find $G_{T_0}(s)$ using $G_{T_1}(s)$.\n",
    "\n",
    "**First find $G_{T_r}(s)$ for $r \\gt 1$:** \n",
    "\n",
    "When $r \\gt 1$, by conditioning on $T_1$, \n",
    "\n",
    "$$\n",
    "\\begin{aligned}\n",
    "  \\displaystyle\n",
    "  \\rho_{0r}(n) &= \\sum_{k=0}^{\\infty}{P(T_r = n | T_1 = k)\\rho_{01}(k)} \\\\\n",
    "               &= \\sum_{k=0}^{n}{P(T_r = n | T_1 = k)\\rho_{01}(k)} \\\\\n",
    "               & = \\sum_{k=0}^{n}{\\rho_{1r}(n-k)\\rho_{01}(k)} \\\\\n",
    "               & = \\sum_{k=0}^{n}{\\rho_{0,r-1}(n-k)\\rho_{01}(k)} \\qquad \\text{Spatial homogeneity}\n",
    "\\end{aligned}\n",
    "$$\n",
    "\n",
    "$$\n",
    "\\begin{aligned}\n",
    "  G_{T_r}(s) &= \\sum_{n=0}^{\\infty} s^n \\rho_{0r}(n) = \\sum_{n=0}^{\\infty} \\sum_{k=0}^{n}  {s^n\\rho_{0,r-1}(n-k)\\rho_{01}(k)} \\\\\n",
    "  &= \\sum_{k=0}^{\\infty} \\sum_{n=k}^{\\infty} {s^k s^{n-k} \\rho_{0,r-1}(n-k)\\rho_{01}(k)} \\\\\n",
    "  &= \\sum_{k=0}^{\\infty} {s^k\\rho_{01}(k)} \\sum_{n=k}^{\\infty}  {s^{n-k}\\rho_{0,r-1}(n-k)} \\\\\n",
    "  &= G_{T_1}(s)G_{T_{r-1}}(s)\n",
    "\\end{aligned}\n",
    "$$\n",
    "\n",
    "By induction: \n",
    "\n",
    "$$\n",
    "G_{T_r}(s)=G_{T_1}^r(s) \\tag{1}\n",
    "$$\n",
    "\n",
    "**Use $G_{T_r}(s)$ to find $G_{T_1}(s)$:** \n",
    "\n",
    "Find $G_{T_1}(s)=\\sum_{n=0}^{\\infty}s^n\\rho_{01}(n)$:\n",
    "\n",
    "$$\n",
    "\\rho_{01}(n) = P_0(T_1 = n | X_1 = 1)p + P_0(T_1 = n | X_1 = -1)q\n",
    "$$\n",
    "\n",
    "- $P_0(T_1 = n | X_1 = 1)$ is 0 if $n=0$ or $n \\ge 2$, and is equal to $1$ when $n=1$.\n",
    "- $P_0(T_1 = n | X_1 = -1)$, has the same probbility that the random walk first reaches state $2$ in $n-1$ times given the initial state is $0$, i.e. $P_0(T_1 = n | X_1 = -1) = P(T_2 = n-1 | X_0 = 0) = \\rho_{02}(n-1)$ for $n \\ge 2$ and $0$ otherwise.\n",
    "\n",
    "Therefore, \n",
    "- when $n=0$, $\\rho_{01}(n) = 0$, \n",
    "- when $n=1$, $\\rho_{01}(n)= p$, \n",
    "- when $n \\ge 2$, $\\rho_{01}(n)=q\\rho_{02}(n-1)$.\n",
    "\n",
    "$$\n",
    "\\begin{aligned}\n",
    "  G_{T_1}(s) &= \\sum_{n=0}^{\\infty}s^n \\rho_{01}(n) \\\\\n",
    "  &= ps + qs\\sum_{n=2}^{\\infty} s^{n-1}\\rho_{02}(n-1) \\\\\n",
    "  &= ps + qs\\sum_{n=1}^{\\infty} s^n\\rho_{02}(n) \\qquad \\text{Change } n-1 \\rightarrow n \\\\\n",
    "  &= ps + qs\\sum_{n=0}^{\\infty} s^n\\rho_{02}(n) \\qquad \\text{using } \\rho_{02}(0) = 0  \\\\\n",
    "  &= ps + qsG_{T_2}(s) \\\\\n",
    "  &= ps + qsG_{T_1}^2(s) \\qquad \\text{using } G_{T_2} = G_{T_1}^2\n",
    "\\end{aligned}\n",
    "$$\n",
    "\n",
    "Solving $qsG_{T_1}^2 - G_{T_1} + ps = 0$, we get:\n",
    "\n",
    "$$\n",
    "\\displaystyle { \n",
    "  G_{T_1} = \\begin{cases}\n",
    "    \\frac{1 + \\sqrt{1-4qps^2}}{2qs} \\\\\n",
    "    \\frac{1 - \\sqrt{1-4qps^2}}{2qs}\n",
    "  \\end{cases}\n",
    " }\n",
    "$$\n",
    "\n",
    "Only one of these two is valid. Note that this solution must also satisfy $G_{T_1}(0) =\\rho_{01}(0) = 0$. The limit $\\lim_{s \\rightarrow 0} \\frac{1 + \\sqrt{1-4qps^2}}{2qs} = \\infty$, therefore the solution should be:\n",
    "\n",
    "$$\n",
    "\\displaystyle{ G_{T_1}(s) = \\frac{1 - \\sqrt{1-4qps^2}}{2qs} }\n",
    "$$\n",
    "\n",
    "Therefore the probability of the first time reaching state $1$ given initial state $0$ is:\n",
    "\n",
    "$$\n",
    "\\begin{aligned}\n",
    "  \\rho_{01} = G_{T_1}(1) &= \\sum_{n=0}^\\infty\\rho_{01}(n) \\\\\n",
    "  &= \\frac{1 - \\sqrt{1-4qp}}{2q} \\\\\n",
    "  &= \\frac{1 - \\sqrt{1-4q+4q^2}}{2q} \\\\\n",
    "  &= \\frac{1 - \\sqrt{(1-2q)^2}}{2q} \\\\\n",
    "  &= \\frac{1 - |1-2q|}{2q} \\\\\n",
    "  &= \\begin{cases}\n",
    "    1 \\qquad \\text{if } q \\le \\frac{1}{2} \\\\\n",
    "    \\frac{p}{q} \\qquad \\text{if } q \\gt \\frac{1}{2}\n",
    "  \\end{cases}\n",
    "\\end{aligned}\n",
    "$$\n",
    "\n",
    "**Find $G_{T_0}(s)$ using $G_{T_1}(s)$:**\n",
    "\n",
    "$$\n",
    "\\begin{aligned}\n",
    "  \\displaystyle\n",
    "    G_{T_0}(s) &= \\sum_{n=0}^{\\infty} s^n \\rho_{00}(n) \\\\\n",
    "    &= \\sum_{n=0}^{\\infty} s^nP(T_0=n|X_0=0) \\\\\n",
    "    &= \\sum_{n=0}^{\\infty} s^n(P(T_0=n|X_1=1)p+P(T_0=n|X_1=-1)q) \\\\\n",
    "    &= \\sum_{n=0}^{\\infty} s^n(P(T_{-1}=n-1|X_0=0)p+P(T_1=n-1|X_0=0)q) \\qquad \\text{By time and spatial property} \\\\\n",
    "    &= \\sum_{n=0}^{\\infty} s^n\\rho_{0,-1}(n-1)p + \\sum_{n=0}^{\\infty} s^n\\rho_{0,1}(n-1)q \\\\\n",
    "    &= spG_{T_{-1}}(s) + sqG_{T_{1}}(s)\n",
    "\\end{aligned}\n",
    "$$\n",
    "\n",
    "But moving from $0$ to $-1$ and moving from $0$ to $1$ is symmetric in distribution with $p, q$ swaped. By swaping the $p$ and $q$ in $G_{T_1}(s) = \\frac{1 - \\sqrt{1-4qps^2}}{2qs}$ we get the value of $G_{T_{-1}}(s)$\n",
    "\n",
    "$$\n",
    "G_{T_{-1}}(s) = \\frac{1 - \\sqrt{1-4qps^2}}{2ps}\n",
    "$$\n",
    "\n",
    "Therefore:\n",
    "\n",
    "$$\n",
    "\\begin{aligned}\n",
    "  \\displaystyle\n",
    "    G_{T_0}(s) &= sp\\frac{1 - \\sqrt{1-4qps^2}}{2ps} + sq\\frac{1 - \\sqrt{1-4qps^2}}{2qs} \\\\\n",
    "    &= 1 - \\sqrt{1-4qps^2} \\\\\n",
    "    \\rho_{00} = G_{T_0}(1) &= 1 - | 1-2q |\n",
    "\\end{aligned}\n",
    "$$\n",
    "\n",
    "\n",
    "When $q=\\frac{1}{2}$, state $0$ is recurrent because:\n",
    "\n",
    "$$\n",
    "\\rho_{00} = 1 \\qquad \\text{if } q=\\frac{1}{2}\n",
    "$$\n",
    "\n",
    "When $q \\ne \\frac{1}{2}$, state $0$ is transient because:\n",
    "\n",
    "$$\n",
    "\\rho_{00} = \\sum_{n=0}^\\infty P(T_0 = n | X_0 = 0) =  \\begin{cases}\n",
    "    2q \\lt 1 & \\text{if } q \\lt \\frac{1}{2} \\\\\n",
    "    2p \\lt 1 & \\text{if } q \\gt \\frac{1}{2}\n",
    "  \\end{cases}\n",
    "$$\n",
    "\n",
    "What about the expected value of $T_0$?\n",
    "\n",
    "\n",
    "Find the derivative of $G_{T_0}(s) = 1 - \\sqrt{1-4pqs^2}$ we get $G'_{T_0}(s) = \\frac{4qps}{\\sqrt{1-4qps^2}}$, hence:\n",
    "\n",
    "When $q=\\frac{1}{2}$:\n",
    "\n",
    "$$\n",
    "E_0(T_0) = G'_{T_0}(1) = \\infty \\qquad \\text{if } q=\\frac{1}{2}\n",
    "$$\n",
    "\n",
    "When $q \\ne \\frac{1}{2}$:\n",
    "\n",
    "$$\n",
    "E_0(T_0) = G'_{T_0}(1) = \\frac{4qp}{\\sqrt{1-4qp}} \\lt \\infty \\qquad \\text{if } q \\ne \\frac{1}{2}\n",
    "$$\n",
    "\n",
    "\n",
    "#### Method 3: Absorbing state\n",
    "\n",
    "Check out the <a href=\"/crypto/blockchain-failure.html\">Bitcoin mining modelling content</a>."
   ]
  }
 ],
 "metadata": {
  "kernelspec": {
   "display_name": "Python 3",
   "language": "python",
   "name": "python3"
  },
  "language_info": {
   "codemirror_mode": {
    "name": "ipython",
    "version": 3
   },
   "file_extension": ".py",
   "mimetype": "text/x-python",
   "name": "python",
   "nbconvert_exporter": "python",
   "pygments_lexer": "ipython3",
   "version": "3.9.5"
  },
  "widgets": {
   "application/vnd.jupyter.widget-state+json": {
    "state": {},
    "version_major": 2,
    "version_minor": 0
   }
  }
 },
 "nbformat": 4,
 "nbformat_minor": 4
}
